pcuic/theories/PCUICValidity.v
@@ -9,9 +9,6 @@ Existing Instance config.default_checker_flags.
 Derive NoConfusion for term.
 Derive Signature for typing cumul.
 
-(* Definition isWfArity Σ (Γ : context) T := *)
-(*   forall ctx s, destArity [] T = Some (ctx, s) -> All_local_env (lift_typing typing) Σ (Γ ,,, ctx). *)
-
 Lemma isWfArity_or_Type_lift Σ n Γ ty (isdecl : n <= #|Γ|):
   wf Σ -> wf_local Σ Γ ->
   isWfArity_or_Type Σ (skipn n Γ) ty ->
@@ -129,6 +126,9 @@ Proof.
   induction u in f, fty, T |- *. simpl. intros. exists T, T. intuition auto. constructor.
   intros Hf Hty. simpl in Hty.
   specialize (IHu _ fty _ Hf) as [T' [U' [[H' H''] H''']]].
+  simpl in Hf.
+  econstructor.
+
 Admitted.
 (*   eapply invert_type_App in H' as (fA & fB & fna & Hf). intuition. *)
 (*   exists (tProd fna fA fB), U'. intuition auto. *)
